src/Language/PlutusIR/Semantics/TypeSafety/SubstitutionPreservesTyping/TypeSubstitution.v
@@ -1,13 +1,17 @@
 Require Import PlutusCert.Language.PlutusIR.
 Import NamedTerm.
 
+Require Import Lists.List.
+Import ListNotations.
+
 Require Import PlutusCert.Language.PlutusIR.Semantics.Static.
 
+Require Import PlutusCert.Util.List.
 
 
 Theorem substituteT_preserves_kinding : forall T Delta X K U L,
-  (X |-> L; Delta) |-* T : K ->
-  empty |-* U : L ->
+  ((X, L) :: Delta) |-* T : K ->
+  [] |-* U : L ->
   Delta |-* (substituteT X U T) : K.
 Proof with eauto with typing.
   induction T.
@@ -22,12 +26,12 @@ Proof with eauto with typing.
       apply eqb_eq in Heqb as Heq.
       subst.
       apply Kinding.weakening_empty.
-      rewrite update_eq in H1.
+      rewrite lookup_eq in H1.
       inversion H1.
       subst...
     + (* X <> Y *)
       apply eqb_neq in Heqb as Hneq.
-      rewrite update_neq in H1...
+      rewrite lookup_neq in H1...
   - (* Ty_Forall *)
     rename b into bX.
     destruct (X =? bX)%string eqn:Heqb.
@@ -35,12 +39,14 @@ Proof with eauto with typing.
       apply eqb_eq in Heqb as Heq.
       subst.
       apply K_Forall...
-      rewrite update_shadow in H4...
+      apply Kinding.weakening with (Delta := ((bX, k) :: (bX, L) :: Delta)).
+      all: auto using cons_shadow.
     + (* X <> bX *)
       apply eqb_neq in Heqb as Hneq.
       apply K_Forall.
       eapply IHT...
-      rewrite update_permute...
+      apply Kinding.weakening with (Delta := (bX, k) :: (X, L) :: Delta)...
+      apply cons_permute...
   - (* Ty_Lam *)  
     rename b into bX.
     destruct (X =? bX)%string eqn:Heqb.
@@ -48,9 +54,14 @@ Proof with eauto with typing.
       apply eqb_eq in Heqb as Heq.
       subst.
       apply K_Lam.
-      rewrite update_shadow in H4...
+      apply Kinding.weakening with (Delta := ((bX, k) :: (bX, L) :: Delta))...
+      apply cons_shadow.
     + (* X <> bX *)
       apply eqb_neq in Heqb as Hneq.
       apply K_Lam.
-      rewrite update_permute in H4...
+      assert (((X, L) :: (bX, k) ::  Delta) |-* T : K2).
+      { apply Kinding.weakening with (Delta' := ((X, L) :: (bX, k) :: Delta)) in H4...
+        apply cons_permute...
+      }
+      idtac...
 Qed.
